@prefix qudt-quantity:  <http://qudt.org/vocab/quantity#> .
@prefix common-core:  <http://test.wmocodes.info/common/schema/core#> .
@prefix qudt:    <http://qudt.org/schema/qudt#> .
@prefix rdfs:    <http://www.w3.org/2000/01/rdf-schema#> .
@prefix rdf:     <http://www.w3.org/1999/02/22-rdf-syntax-ns#> .
@prefix dc:      <http://purl.org/dc/elements/1.1/> .
@prefix foaf:    <http://xmlns.com/foaf/0.1/> .
@prefix qudt-unit:  <http://qudt.org/vocab/unit#> .
@prefix common-units:  <http://test.wmocodes.info/common/schema/units#> .
@prefix dct:     <http://purl.org/dc/terms/> .
@prefix reg:     <http://purl.org/linked-data/registry#> .
@prefix owl:     <http://www.w3.org/2002/07/owl#> .
@prefix xsd:     <http://www.w3.org/2001/XMLSchema#> .
@prefix skos:    <http://www.w3.org/2004/02/skos/core#> .
@prefix ldp:     <http://www.w3.org/ns/ldp#> .

<_dewPointTemperature>
    a reg:RegisterItem ;
    common-core:Status common-core:statusValidation ;
    reg:definition
        [ reg:entity <dewPointTemperature> ] ;
    reg:itemClass qudt:QuantityKind , qudt:ThermodynamicsQuantityKind ;
    reg:notation "dewPointTemperature" ;
    reg:register <http://test.wmocodes.info/common/c-15/me> ;
    reg:status reg:statusExperimental ;
    reg:submitter
        [ foaf:name "Jeremy Tandy" ;
          foaf:openid <https://profiles.google.com/101323394574484397758>
        ] ;
    .
<dewPointTemperature>
    a qudt:QuantityKind , qudt:ThermodynamicsQuantityKind ;
    rdfs:label "Dew-point temperature"@en ;
    dct:description "The temperature to which a given air parcel must be cooled at constant pressure and constant water vapor content in order for saturation to occur."@en ;
    qudt:generalization qudt-quantity:ThermodynamicTemperature ;
    .
<_airTemperature>
    a reg:RegisterItem ;
    common-core:Status common-core:statusValidation ;
    reg:definition
        [ reg:entity <airTemperature> ] ;
    reg:itemClass qudt:QuantityKind , qudt:ThermodynamicsQuantityKind ;
    reg:notation "airTemperature" ;
    reg:register <http://test.wmocodes.info/common/c-15/me> ;
    reg:status reg:statusExperimental ;
    reg:submitter
        [ foaf:name "Jeremy Tandy" ;
          foaf:openid <https://profiles.google.com/101323394574484397758>
        ] ;
    .
<airTemperature>
    a qudt:QuantityKind , qudt:ThermodynamicsQuantityKind ;
    rdfs:label "Air temperature"@en ;
    dct:description "The temperature indicated by a thermometer exposed to the air in a place sheltered from direct solar radiation."@en ;
    qudt:generalization qudt-quantity:ThermodynamicTemperature ;
    .
<_uvIndex>
    a reg:RegisterItem ;
    common-core:Status common-core:statusValidation ;
    reg:definition
        [ reg:entity <uvIndex> ] ;
    reg:itemClass qudt:QuantityKind ;
    reg:notation "uvIndex" ;
    reg:register <http://test.wmocodes.info/common/c-15/me> ;
    reg:status reg:statusExperimental ;
    reg:submitter
        [ foaf:name "Jeremy Tandy" ;
          foaf:openid <https://profiles.google.com/101323394574484397758>
        ] ;
    .
<uvIndex>
    a qudt:QuantityKind ;
    rdfs:label "UV index"@en ;
    dct:description "Global Solar UVI is formulated using the International Commission on Illumination (CIE) reference action spectrum for UV-induced erythema on the human skin (ISO 17166:1999/CIE S 007/E-1998). It is a measure of the UV radiation that is relevant to and defined for a horizontal surface."@en ;
    qudt:generalization qudt-quantity:DimensionlessRatio ;
    .
<_horizontalVisibility>
    a reg:RegisterItem ;
    common-core:Status common-core:statusValidation ;
    reg:definition [ reg:entity <horizontalVisibility> ] ;
    reg:itemClass qudt:QuantityKind , qudt:SpaceAndTimeQuantityKind ;
    reg:notation "horizontalVisibility" ;
    reg:register <http://test.wmocodes.info/common/c-15/me> ;
    reg:status reg:statusExperimental ;
    reg:submitter
        [ foaf:name "Jeremy Tandy" ;
          foaf:openid <https://profiles.google.com/101323394574484397758>
        ] ;
    .
<horizontalVisibility>
    a qudt:QuantityKind , qudt:SpaceAndTimeQuantityKind ;
    rdfs:label "Horizontal visibility"@en ;
    dct:description "The greatest distance determined in the horizontal plane at the ground surface that prominent objects can be seen and identified by unaided, normal eyes."@en ;
    qudt:generalization qudt-quantity:Length ;
    .
<_maximumDiameterOfHailstones>
    a reg:RegisterItem ;
    common-core:Status common-core:statusValidation ;
    reg:definition [ reg:entity <maximumDiameterOfHailstones> ] ;
    reg:itemClass qudt:QuantityKind , qudt:SpaceAndTimeQuantityKind ;
    reg:notation "maximumDiameterOfHailstones" ;
    reg:register <http://test.wmocodes.info/common/c-15/me> ;
    reg:status reg:statusExperimental ;
    reg:submitter
        [ foaf:name "Jeremy Tandy" ;
          foaf:openid <https://profiles.google.com/101323394574484397758>
        ] ;
    .
<maximumDiameterOfHailstones>
    a qudt:QuantityKind , qudt:SpaceAndTimeQuantityKind ;
    rdfs:label "Maximum diameter of hailstones"@en ;
    dct:description "Maximum diameter (size) of hailstone (observed)."@en ;
    qudt:generalization qudt-quantity:Length ;
    .
<_windSpeed>
    a reg:RegisterItem ;
    common-core:Status common-core:statusValidation ;
    reg:definition [ reg:entity <windSpeed> ] ;
    reg:itemClass qudt:QuantityKind , qudt:SpaceAndTimeQuantityKind ;
    reg:notation "windSpeed" ;
    reg:register <http://test.wmocodes.info/common/c-15/me> ;
    reg:status reg:statusExperimental ;
    reg:submitter
        [ foaf:name "Jeremy Tandy" ;
          foaf:openid <https://profiles.google.com/101323394574484397758>
        ] ;
    .
<windSpeed>
    a qudt:QuantityKind , qudt:SpaceAndTimeQuantityKind ;
    rdfs:label "Wind speed"@en ;
    dct:description "Ratio of the distance covered by the air to the time taken to cover it. The instantaneous speed corresponds to the case of an infinitely small time interval. The mean speed corresponds to the case of a finite time interval. It is one component of wind velocity, the other being wind direction)."@en ;
    qudt:generalization qudt-quantity:LinearVelocity ;
    .
<_windDirection>
    a reg:RegisterItem ;
    common-core:Status common-core:statusValidation ;
    reg:definition [ reg:entity <windDirection> ] ;
    reg:itemClass qudt:QuantityKind , qudt:SpaceAndTimeQuantityKind ;
    reg:notation "windDirection" ;
    reg:register <http://test.wmocodes.info/common/c-15/me> ;
    reg:status reg:statusExperimental ;
    reg:submitter
        [ foaf:name "Jeremy Tandy" ;
          foaf:openid <https://profiles.google.com/101323394574484397758>
        ] ;
    .
<windDirection>
    a qudt:QuantityKind , qudt:SpaceAndTimeQuantityKind ;
    rdfs:label "Wind direction"@en ;
    dct:description "Direction from which wind is blowing."@en ;
    qudt:generalization qudt-quantity:PlaneAngle ;
    .
<_maximumWindGustSpeed>
    a reg:RegisterItem ;
    common-core:Status common-core:statusValidation ;
    reg:definition [ reg:entity <maximumWindGustSpeed> ] ;
    reg:itemClass qudt:QuantityKind , qudt:SpaceAndTimeQuantityKind ;
    reg:notation "maximumWindGustSpeed" ;
    reg:register <http://test.wmocodes.info/common/c-15/me> ;
    reg:status reg:statusExperimental ;
    reg:submitter
        [ foaf:name "Jeremy Tandy" ;
          foaf:openid <https://profiles.google.com/101323394574484397758>
        ] ;
    .
<maximumWindGustSpeed>
    a qudt:QuantityKind , qudt:SpaceAndTimeQuantityKind ;
    rdfs:label "Wind speed (gust)"@en ;
    dct:description "Nominal maximum speed of wind during a given period; usually determined as an mean wind speed over a short duration (e.g. 1-minute) within a longer period (e.g. 10-minutes)."@en ;
    qudt:generalization qudt-quantity:LinearVelocity ;
    .
<_totalPrecipitationRate>
    a reg:RegisterItem ;
    common-core:Status common-core:statusValidation ;
    reg:definition [ reg:entity <totalPrecipitationRate> ] ;
    reg:itemClass qudt:QuantityKind , qudt:MechanicsQuantityKind ;
    reg:notation "totalPrecipitationRate" ;
    reg:register <http://test.wmocodes.info/common/c-15/me> ;
    reg:status reg:statusExperimental ;
    reg:submitter
        [ foaf:name "Jeremy Tandy" ;
          foaf:openid <https://profiles.google.com/101323394574484397758>
        ] ;
    .
<totalPrecipitationRate>
    a qudt:QuantityKind , qudt:MechanicsQuantityKind ;
    rdfs:label "Total precipitation rate"@en ;
    dct:description "Rate of total precipitation (e.g. combination of convective and large-scale precipitation of all types)."@en ;
    qudt:generalization qudt-quantity:MassPerAreaTime ;
    .
<_totalPrecipitation>
    a reg:RegisterItem ;
    common-core:Status common-core:statusValidation ;
    reg:definition [ reg:entity <totalPrecipitation> ] ;
    reg:itemClass qudt:QuantityKind , qudt:MechanicsQuantityKind ;
    reg:notation "totalPrecipitation" ;
    reg:register <http://test.wmocodes.info/common/c-15/me> ;
    reg:status reg:statusExperimental ;
    reg:submitter
        [ foaf:name "Jeremy Tandy" ;
          foaf:openid <https://profiles.google.com/101323394574484397758>
        ] ;
    .
<totalPrecipitation>
    a qudt:QuantityKind , qudt:MechanicsQuantityKind ;
    rdfs:label "Total precipitation"@en ;
    dct:description "Total amount of precipitation measured over a defined period."@en ;
    qudt:generalization qudt-quantity:MassPerArea ;
    .
<_snowDepthWaterEquivalent>
    a reg:RegisterItem ;
    common-core:Status common-core:statusValidation ;
    reg:definition [ reg:entity <snowDepthWaterEquivalent> ] ;
    reg:itemClass qudt:QuantityKind , qudt:SpaceAndTimeQuantityKind ;
    reg:notation "snowDepthWaterEquivalent" ;
    reg:register <http://test.wmocodes.info/common/c-15/me> ;
    reg:status reg:statusExperimental ;
    reg:submitter
        [ foaf:name "Jeremy Tandy" ;
          foaf:openid <https://profiles.google.com/101323394574484397758>
        ] ;
    .
<snowDepthWaterEquivalent>
    a qudt:QuantityKind , qudt:SpaceAndTimeQuantityKind ;
    rdfs:label "Snow depth water equivelant"@en ;
    dct:description "Depth of lying snow expressed as measure of equivalent depth of water."@en ;
    qudt:generalization qudt-quantity:Length ;
    .
<_totalSnowDepth>
    a reg:RegisterItem ;
    common-core:Status common-core:statusValidation ;
    reg:definition [ reg:entity <totalSnowDepth> ] ;
    reg:itemClass qudt:QuantityKind , qudt:SpaceAndTimeQuantityKind ;
    reg:notation "totalSnowDepth" ;
    reg:register <http://test.wmocodes.info/common/c-15/me> ;
    reg:status reg:statusExperimental ;
    reg:submitter
        [ foaf:name "Jeremy Tandy" ;
          foaf:openid <https://profiles.google.com/101323394574484397758>
        ] ;
    .
<totalSnowDepth>
    a qudt:QuantityKind , qudt:SpaceAndTimeQuantityKind ;
    rdfs:label "Total snow depth"@en ;
    dct:description "Depth of lying snow."@en ;
    qudt:generalization qudt-quantity:Length ;
    .
<_pressureTendency>
    a reg:RegisterItem ;
    common-core:Status common-core:statusValidation ;
    reg:definition [ reg:entity <pressureTendency> ] ;
    reg:itemClass qudt:QuantityKind , qudt:MechanicsQuantityKind ;
    reg:notation "pressureTendency" ;
    reg:register <http://test.wmocodes.info/common/c-15/me> ;
    reg:status reg:statusExperimental ;
    reg:submitter
        [ foaf:name "Jeremy Tandy" ;
          foaf:openid <https://profiles.google.com/101323394574484397758>
        ] ;
    .
<pressureTendency>
    a qudt:QuantityKind , qudt:MechanicsQuantityKind ;
    rdfs:label "Pressure tendency"@en ;
    dct:description "Rate of change of atmospheric pressure with respect to time."@en ;
    qudt:generalization qudt-quantity:ForcePerAreaTime ;
    .
<_pressureReducedToMeanSeaLevel>
    a reg:RegisterItem ;
    common-core:Status common-core:statusValidation ;
    reg:definition [ reg:entity <pressureReducedToMeanSeaLevel> ] ;
    reg:itemClass qudt:QuantityKind , qudt:MechanicsQuantityKind ;
    reg:notation "pressureReducedToMeanSeaLevel" ;
    reg:register <http://test.wmocodes.info/common/c-15/me> ;
    reg:status reg:statusExperimental ;
    reg:submitter
        [ foaf:name "Jeremy Tandy" ;
          foaf:openid <https://profiles.google.com/101323394574484397758>
        ] ;
    .
<pressureReducedToMeanSeaLevel>
    a qudt:QuantityKind , qudt:MechanicsQuantityKind ;
    rdfs:label "Pressure reduced to mean sea-level (MSLP)"@en ;
    dct:description "The atmospheric pressure at mean sea level, either directly measured or, most commonly, empirically determined from the observed station pressure."@en ;
    qudt:generalization qudt-quantity:ForcePerArea ;
    .
<_geometricHeight>
    a reg:RegisterItem ;
    common-core:Status common-core:statusValidation ;
    reg:definition [ reg:entity <geometricHeight> ] ;
    reg:itemClass qudt:QuantityKind , qudt:SpaceAndTimeQuantityKind ;
    reg:notation "geometricHeight" ;
    reg:register <http://test.wmocodes.info/common/c-15/me> ;
    reg:status reg:statusExperimental ;
    reg:submitter
        [ foaf:name "Jeremy Tandy" ;
          foaf:openid <https://profiles.google.com/101323394574484397758>
        ] ;
    .
<geometricHeight>
    a qudt:QuantityKind , qudt:SpaceAndTimeQuantityKind ;
    rdfs:label "Geometric height"@en ;
    dct:description "Vertical distance (Z) of a level, a point or an object considered as a point, measured from mean sea level. (Also known as geometric altitude)."@en ;
    qudt:generalization qudt-quantity:Length ;
    .
<_altimeterSettingQnh>
    a reg:RegisterItem ;
    common-core:Status common-core:statusValidation ;
    reg:definition [ reg:entity <altimeterSettingQnh> ] ;
    reg:itemClass qudt:QuantityKind , qudt:MechanicsQuantityKind ;
    reg:notation "altimeterSettingQnh" ;
    reg:register <http://test.wmocodes.info/common/c-15/me> ;
    reg:status reg:statusExperimental ;
    reg:submitter
        [ foaf:name "Jeremy Tandy" ;
          foaf:openid <https://profiles.google.com/101323394574484397758>
        ] ;
    .
<altimeterSettingQnh>
    a qudt:QuantityKind , qudt:MechanicsQuantityKind ;
    rdfs:label "Altimeter setting (QNH)"@en ;
    dct:description "Altitude setting (also known as QNH) is defined as barometric pressure adjusted to sea level. It is a pressure setting used by pilots, air traffic control (ATC), and low frequency weather beacons to refer to the barometric setting which, when set on an aircraft's altimeter, will cause the altimeter to read altitude above mean sea level within a certain defined region. [note inclusion of this physical quantity within ‘meteorology’ discipline, as opposed to ‘aeronautical meteorology’, due to legacy compatibility with GRIB code-tables – however, GRIB does not contain an ‘aeronautical meteorology’ discipline]"@en ;
    qudt:generalization qudt-quantity:ForcePerArea ;
    .
<_heightOfBaseOfCloud>
    a reg:RegisterItem ;
    common-core:Status common-core:statusValidation ;
    reg:definition [ reg:entity <heightOfBaseOfCloud> ] ;
    reg:itemClass qudt:QuantityKind , qudt:SpaceAndTimeQuantityKind ;
    reg:notation "heightOfBaseOfCloud" ;
    reg:register <http://test.wmocodes.info/common/c-15/me> ;
    reg:status reg:statusExperimental ;
    reg:submitter
        [ foaf:name "Jeremy Tandy" ;
          foaf:openid <https://profiles.google.com/101323394574484397758>
        ] ;
    .
<heightOfBaseOfCloud>
    a qudt:QuantityKind , qudt:SpaceAndTimeQuantityKind ;
    rdfs:label "Height of base of cloud"@en ;
    dct:description "For a given cloud or cloud layer, vertical distance (measured from local ground surface) of the lowest level in the atmosphere at which the air contains a perceptible quantity of cloud particles."@en ;
    qudt:generalization qudt-quantity:Length ;
    .
<_cloudType>
    a reg:RegisterItem ;
    common-core:Status common-core:statusValidation ;
    reg:definition [ reg:entity <cloudType> ] ;
    reg:itemClass owl:Class ;
    reg:notation "cloudType" ;
    reg:register <http://test.wmocodes.info/common/c-15/me> ;
    reg:status reg:statusExperimental ;
    reg:submitter
        [ foaf:name "Jeremy Tandy" ;
          foaf:openid <https://profiles.google.com/101323394574484397758>
        ] ;
    .
<cloudType>
    a owl:Class ;
    rdfs:label "Cloud type"@en ;
    dct:description "Genus of cloud."@en ;
    rdfs:subClassOf skos:Concept ;
    .
<_meteorologicalFeature>
    a reg:RegisterItem ;
    common-core:Status common-core:statusValidation ;
    reg:definition [ reg:entity <meteorologicalFeature> ] ;
    reg:itemClass owl:Class ;
    reg:notation "meteorologicalFeature" ;
    reg:register <http://test.wmocodes.info/common/c-15/me> ;
    reg:status reg:statusExperimental ;
    reg:submitter
        [ foaf:name "Jeremy Tandy" ;
          foaf:openid <https://profiles.google.com/101323394574484397758>
        ] ;
    .
<meteorologicalFeature>
    a owl:Class ;
    rdfs:label "Meteorological feature"@en ;
    dct:description "Class of meteorological feature (e.g. front, cloud, tropical cyclone, jet-stream etc.)."@en ;
    rdfs:subClassOf skos:Concept ;
    .
<_characteristicOfPressureTendency>
    a reg:RegisterItem ;
    common-core:Status common-core:statusValidation ;
    reg:definition [ reg:entity <characteristicOfPressureTendency> ] ;
    reg:itemClass owl:Class ;
    reg:notation "characteristicOfPressureTendency" ;
    reg:register <http://test.wmocodes.info/common/c-15/me> ;
    reg:status reg:statusExperimental ;
    reg:submitter
        [ foaf:name "Jeremy Tandy" ;
          foaf:openid <https://profiles.google.com/101323394574484397758>
        ] ;
    .
<characteristicOfPressureTendency>
    a owl:Class ;
    rdfs:label "Characteristic of pressure tendency"@en ;
    rdfs:subClassOf skos:Concept ;
    .